core/AssertionLang.v
@@ -1,0 +1,107 @@
+Require Import Coq.ssr.ssrbool.
+Require Import Coq.ssr.ssreflect.
+Require Import Poulet4.Typed.
+Require Import Poulet4.Syntax.
+Require Import Poulet4.Semantics.
+Require Import ProD3.core.Coqlib.
+
+Section AssertionLang.
+
+Context {tags_t: Type} {tags_t_inhabitant : Inhabitant tags_t}.
+Notation Val := (@ValueBase tags_t).
+
+Notation ident := (P4String.t tags_t).
+Notation path := (list ident).
+Notation P4Int := (P4Int.t tags_t).
+Notation P4String := (P4String.t tags_t).
+Notation signal := (@signal tags_t).
+
+Context `{@Target tags_t (@Expression tags_t)}.
+
+Definition assertion := list (@Locator tags_t * Val).
+
+Variable this : path.
+
+Definition satisfies_unit (st : state) (a_unit : @Locator tags_t * Val) : Prop :=
+  let (loc, v) := a_unit in
+  loc_to_val this loc st = Some v.
+
+Definition satisfies (st : state) (a : assertion) : Prop :=
+  fold_left and (map (satisfies_unit st) a) True.
+
+Definition to_shallow_assertion (a : assertion) : state -> Prop :=
+  fun st => satisfies st a.
+
+Definition no_overlapping_unit_unit (a_unit1 a_unit2 : @Locator tags_t * Val) : bool :=
+  let (loc1, _) := a_unit1 in
+  let (loc2, _) := a_unit2 in
+  match loc1, loc2 with
+  | LInstance p1, LInstance p2 => ~~ (path_equivb p1 p2)
+  | _, _ => false
+  end.
+
+Fixpoint no_overlapping_unit (a_unit : @Locator tags_t * Val) (a : assertion) : bool :=
+  match a with
+  | hd :: tl => no_overlapping_unit_unit a_unit hd && no_overlapping_unit a_unit tl
+  | [] => true
+  end.
+
+Fixpoint no_overlapping (a : assertion) : bool :=
+  match a with
+  | hd :: tl => no_overlapping_unit hd tl && no_overlapping tl
+  | [] => true
+  end.
+
+Definition locator_equiv (loc1 loc2 : @Locator tags_t) : bool :=
+  match loc1, loc2 with
+  | LInstance p1, LInstance p2 => path_equivb p1 p2
+  | LGlobal p1, LGlobal p2 => path_equivb p1 p2
+  | _, _ => false
+  end.
+
+Fixpoint update_val_by_loc (a : assertion) (loc : Locator) (v : Val) : assertion :=
+  match a with
+  | (hd_loc, hd_v) :: tl =>
+      if locator_equiv loc hd_loc then
+        (hd_loc, v) :: tl
+      else
+        (hd_loc, hd_v) :: update_val_by_loc tl loc v
+  | [] => [(loc, v)]
+  end.
+
+Definition is_instance (loc : @Locator tags_t) : bool :=
+  match loc with
+  | LInstance _ => true
+  | LGlobal _ => false
+  end.
+
+(* Lemma update_val_by_loc_sound : forall st a loc v,
+  no_overlapping a ->
+  is_instance loc = true ->
+  to_shallow_assertion a st ->
+  to_shallow_assertion (update_val_by_loc a loc v) (Semantics.update_val_by_loc this st loc v).
+Proof.
+  intros * H_no_overlapping H_is_instance H_pre.
+  destruct loc; only 1 : inversion H_is_instance.
+  unfold to_shallow_assertion in *.
+  induction a; intros.
+  - destruct st. simpl. unfold satisfies. simpl. repeat split.
+    unfold loc_to_val. simpl.
+    replace (PathMap.get (this ++ p) (PathMap.set (this ++ p) v m)) with (Some v) by admit.
+    reflexivity.
+  - assert (satisfies (Semantics.update_val_by_loc this st (LInstance p) v)
+        (update_val_by_loc a0 (LInstance p) v)). {
+      apply IHa.
+      - simpl in H_no_overlapping. Search reflect and. move /andP : H_no_overlapping => H_no_overlapping. apply H_no_overlapping. *)
+
+End AssertionLang.
+
+
+
+
+
+
+
+
+
+
