core/Coqlib.v
@@ -1,0 +1,4 @@
+Require Export Coq.Lists.List.
+Export ListNotations.
+
+Notation "~~" := negb.
