core/Hoare.v
@@ -1,0 +1,129 @@
+Require Import Poulet4.Typed.
+Require Import Poulet4.Syntax.
+Require Import Poulet4.Semantics.
+Require Import ProD3.core.Coqlib.
+
+Section Hoare.
+
+Context {tags_t: Type} {tags_t_inhabitant : Inhabitant tags_t}.
+Notation Val := (@ValueBase tags_t).
+
+Notation ident := (P4String.t tags_t).
+Notation path := (list ident).
+Notation P4Int := (P4Int.t tags_t).
+Notation P4String := (P4String.t tags_t).
+Notation signal := (@signal tags_t).
+
+Context `{@Target tags_t (@Expression tags_t)}.
+
+Variable ge : (@genv tags_t).
+Variable ge_typ : (@genv_typ tags_t).
+Variable ge_senum : (@genv_senum tags_t).
+Variable inst_m : (@inst_mem tags_t).
+
+Definition assertion := state -> Prop.
+
+Definition hoare_stmt (p : path) (pre : assertion) (stmt : Statement) (post : assertion) :=
+  forall st st' sig,
+    pre st ->
+    exec_stmt ge ge_typ ge_senum p inst_m st stmt st' sig ->
+    sig = SContinue /\ post st'.
+
+Definition hoare_block (p : path) (pre : assertion) (block : Block) (post : assertion) :=
+  forall st st' sig,
+    pre st ->
+    exec_block ge ge_typ ge_senum p inst_m st block st' sig ->
+    sig = SContinue /\ post st'.
+
+Definition hoare_call (p : path) (pre : assertion) (expr : Expression) (post : assertion) :=
+  forall st st' sig,
+    pre st ->
+    exec_call ge ge_typ ge_senum p inst_m st expr st' sig ->
+    sig = SContinue /\ post st'.
+
+Definition arg_assertion := list Val -> state -> Prop.
+
+Definition hoare_func (p : path) (pre : arg_assertion) (func : @fundef tags_t) (targs : list P4Type) (post : arg_assertion) :=
+  forall st inargs st' outargs sig,
+    pre inargs st ->
+    exec_func ge ge_typ ge_senum p inst_m st func targs inargs st' outargs sig ->
+    sig = SContinue /\ post outargs st'.
+
+Section DeepEmbeddedHoare.
+
+Definition implies (pre post : assertion) :=
+  forall st, pre st -> post st.
+
+Inductive deep_hoare_stmt : path -> assertion -> Statement -> assertion -> Prop :=
+  | deep_hoare_stmt_intro : forall p pre stmt post,
+      hoare_stmt p pre stmt post ->
+      deep_hoare_stmt p pre stmt post.
+
+Inductive deep_hoare_block : path -> assertion -> Block -> assertion -> Prop :=
+  | deep_hoare_block_nil : forall p pre post,
+      implies pre post ->
+      deep_hoare_block p pre BlockNil post
+  | deep_hoare_block_cons : forall p pre stmt mid block post,
+      deep_hoare_stmt p pre stmt mid ->
+      deep_hoare_block p mid block post ->
+      deep_hoare_block p pre (BlockCons stmt block) post.
+
+Definition hoare_eval_expr (p : path) (pre : assertion) (expr : Expression) (v : Val) : Prop :=
+  forall st,
+    pre st ->
+    exec_expr ge_typ ge_senum p st expr v.
+
+Definition hoare_eval_lvalue_expr (p : path) (pre : assertion) (expr : Expression) (lv : Lval) : Prop :=
+  forall st,
+    pre st ->
+    exec_lvalue_expr ge_typ ge_senum p st expr lv SContinue.
+
+Inductive deep_hoare_call : path -> assertion -> Expression -> assertion -> Prop :=
+  | deep_hoare_call_intro : forall p pre expr post,
+      hoare_call p pre expr post ->
+      deep_hoare_call p pre expr post.
+
+Fixpoint _in (x : ident) (al : list ident) : bool :=
+  match al with
+  | y :: al => P4String.equivb x y || _in x al
+  | [] => false
+  end.
+
+Fixpoint no_dup (al : list ident) : bool :=
+  match al with
+  | x :: al => ~~(_in x al) && no_dup al
+  | [] => true
+  end.
+
+Inductive deep_hoare_func : path -> arg_assertion -> @fundef tags_t -> list P4Type -> arg_assertion -> Prop :=
+  | deep_hoare_func_internal : forall p pre func targs post,
+      hoare_func p pre func targs post ->
+      deep_hoare_func p pre func targs post.
+(*   | deep_hoare_func_intro : forall p pre func targs post,
+      hoare_func p pre func targs post ->
+      deep_hoare_func p pre func targs post. *)
+
+(* FInternal : list (P4String.t tags_t * direction) -> Block -> Block -> fundef *)
+
+End DeepEmbeddedHoare.
+
+End Hoare.
+
+
+
+
+
+
+
+
+
+
+
+
+
+
+
+
+
+
+
